Coq/common.v
@@ -5,28 +5,30 @@ Require Import List.
 Inductive var : Type :=
 | bind : nat -> var.
 
-Class Eqb (A : Type) :=
+Class Eq (A : Type) :=
   {eqb : A -> A -> bool;
    eqb_refl : forall a, eqb a a = true;
    eqb_sym : forall a1 a2, eqb a1 a2 = eqb a2 a1;
-   eqb_eq : forall a1 a2, eqb a1 a2 = true ->
-                     a1 = a2;
+   eqb_eqp : forall a1 a2, eqb a1 a2 = true ->
+                      a1 = a2;
+   eqb_neq : forall a1 a2, eqb a1 a2 = false ->
+                      a1 <> a2;
    neq_eqb : forall a1 a2, a1 <> a2 ->
                       eqb a1 a2 = false;
-   eqb_neq : forall a1 a2, eqb a1 a2 = false ->
-                      a1 <> a2}.
+   eq_dec : forall (a1 a2 : A), {a1 = a2} + {a1 <> a2}}.
 
-Instance nat_Eqb : Eqb nat :=
+Instance nat_Eq : Eq nat :=
   {eqb n m := n =? m;
    eqb_refl := Nat.eqb_refl;
-   eqb_sym := Nat.eqb_sym}.
+   eqb_sym := Nat.eqb_sym;
+   eq_dec := Nat.eq_dec}.
 Proof.
   intros; apply beq_nat_eq; auto.
   apply Nat.eqb_neq.
   apply Nat.eqb_neq.
 Defined.
 
-Instance var_Eqb : Eqb var :=
+Instance var_Eq : Eq var :=
   {eqb x y :=
      match x, y with
      | bind n, bind m => n =? m
@@ -43,39 +45,93 @@ Proof.
   intros;
     destruct a1;
     destruct a2;
-    rewrite Nat.eqb_neq;
+    rewrite Nat.eqb_neq in H;
     crush.
   intros;
     destruct a1;
     destruct a2;
-    rewrite Nat.eqb_neq in H;
+    rewrite Nat.eqb_neq;
+    crush.
+  intros x y;
+    destruct x as [n];
+    destruct y as [m];
+    destruct (Nat.eq_dec n m) as [Heq|Hneq];
+    subst;
+    auto;
+    right;
     crush.
 Defined.
 
-Definition total_map (A B : Type) `{Eqb A} := A -> B.
+(*Section partial_maps.
 
-Definition t_empty {A B : Type} `{Eqb A} (b : B) : total_map A B := (fun _ => b).
+  Set Implicit Arguments.
 
-Definition t_update {A B : Type} `{Eqb A} (map : total_map A B) (a : A)(b : B) :=
+  Variables A B : Set.
+           
+  Inductive partial_map : Set :=
+  | empty : partial_map
+  | update : A -> B -> partial_map -> partial_map.
+
+  Fixpoint pmap `{Eq A} (m : partial_map)(a : A) : option B :=
+    match m with
+    | empty => None
+    | update a' b m' => if (eqb a a')
+                       then Some b
+                       else pmap m' a
+    end.
+  Unset Implicit Arguments.
+
+End partial_maps.*)
+
+Definition total_map (A B : Type) `{Eq A} := A -> B.
+
+Definition t_empty {A B : Type} `{Eq A} (b : B) : total_map A B := (fun _ => b).
+
+Definition t_update {A B : Type} `{Eq A} (map : total_map A B) (a : A)(b : B) :=
   fun x => if (eqb x a) then b else map x.
 
 (*Definition t_compose {A B C : Type} `{Eq A} (map1 map2 : total_map)*)
 
-Definition partial_map (A B : Type) `{Eqb A} := total_map A (option B).
+Definition partial_map (A B : Type) `{Eq A} := total_map A (option B).
 
-Definition empty {A B : Type} `{Eqb A} : partial_map A B := t_empty None.
+Definition empty {A B : Type} `{Eq A} : partial_map A B := t_empty None.
 
-Definition update {A B : Type} `{Eqb A} (a : A) (b : B) (map : partial_map A B) :=
+Definition update {A B : Type} `{Eq A} (a : A) (b : B) (map : partial_map A B) :=
   t_update map a (Some b).
 
 Definition compose
-           {A B C : Type} `{Eqb A} `{Eqb B}
+           {A B C : Type} `{Eq A} `{Eq B}
            (map1 : partial_map A B)
            (map2 : partial_map B C) : partial_map A C :=
   fun a => match map1 a with
         | None => None
         | Some b => map2 b
         end.
+
+(*Fixpoint compose
+         {A B C : Set} `{Eq A} `{Eq B}
+         (m1 : partial_map A B)(m2 : partial_map B C) : partial_map A C :=
+  match m1 with
+  | empty _ _ => empty _ _
+  | update a b m => match (pmap m2 b) with
+                   | None => compose m m2
+                   | Some c => update a c (compose m m2)
+                   end
+  end.*)
+
+Definition extend {A B : Type} `{Eq A} (M1 M2 : partial_map A B) : partial_map A B :=
+  fun a =>
+    match M1 a with
+    | None => M2 a
+    | _ => M1 a
+    end.
+
+Inductive finite {A B : Type}`{Eq A} : partial_map A B -> Prop :=
+| fin_empty : finite empty
+| fin_update : forall a b m, finite m ->
+                        finite (update a b m).
+
+Hint Constructors finite.
 
 Class Mappable (A B C : Type) :=
   map : A -> B -> C.
