Coq/fundamental_properties.v
@@ -1,0 +1,1630 @@
+Require Import common.
+Require Import loo_def.
+Require Import chainmail.
+Require Import List.
+Require Import CpdtTactics.
+Require Import Coq.Logic.FunctionalExtensionality.
+
+(** #<h1># Basic Arithmetic Assertions: #</h1># *)
+
+(** Law of the Excluded Middle: *)
+Parameter excluded_middle : forall P, P \/ ~P.
+
+Lemma prop_not_and_distr :
+  forall A B, ~(A /\ B) -> ~A \/ ~B.
+Proof.
+  intros.
+  destruct (excluded_middle A);
+    destruct (excluded_middle B);
+    crush.
+Qed.
+
+Lemma prop_implies_not :
+  forall (A B : Prop), (A -> ~B) -> (B -> ~A).
+Proof.
+  crush.
+Qed.
+
+Lemma prop_not_sat_and_distr :
+  forall M1 M2 σ A1 A2, ~M1 ⦂ M2 ◎ σ ⊨ (a_and A1 A2) ->
+                   (~M1 ⦂ M2 ◎ σ ⊨ A1) \/
+                   (~ M1 ⦂ M2 ◎ σ ⊨ A2).
+Proof.
+  intros;
+    apply prop_not_and_distr;
+    intros Hcontra;
+    destruct Hcontra as [Ha Hb];
+    crush.
+Qed.
+
+Lemma forall_exists_neg :
+  forall {A : Type} P, (forall (x : A), ~ P) ->
+                  ~ (exists (a : A), P).
+Proof.
+  intros; crush.
+Qed.
+
+Lemma exists_neg_forall :
+  forall {A : Type} (P : A -> Prop),
+    ~ (exists (a : A), P a) ->
+    (forall (a : A), ~ P a).
+Proof.
+  intros; intros Hcontra.
+  contradiction H.
+  exists a; auto.
+Qed.
+
+Lemma reduction_preserves_well_formed_heap :
+  forall M σ1 σ2, M ∙ σ1 ⤳ σ2 ->
+             χ_wf M (fst σ1) ->
+             χ_wf M (fst σ2).
+Proof.
+  intros M σ1 σ2 Hred;
+    induction Hred;
+    intros;
+    try solve [crush];
+    subst;
+    apply heap_wf;
+    intros;
+    subst.
+
+  (*field assign reduce*)
+  simpl in H.
+  unfold update, t_update in H.
+  destruct (eq_dec α0 α) as [Heq|Hneq];
+    [subst; rewrite eqb_refl in H; auto
+    |apply neq_eqb in Hneq; rewrite Hneq in H;
+     inversion H11; subst; apply (H7 α0); auto].
+  inversion H11; subst.
+  destruct (H7 α o (cname o)) as [CDef Hwf]; auto;
+    destruct Hwf as [Hwf1 Hwf2];
+    destruct Hwf2 as [Hwf2 Hwf3].
+  exists CDef; split;
+    [inversion H; subst; auto
+    |split;
+     [intros
+     |inversion H; subst; auto]].
+  inversion H; subst; simpl.
+  destruct (eq_dec f0 f) as [Heq|Hneq];
+    [destruct f0; subst; rewrite <- beq_nat_refl; exists (v_addr α'); auto
+    |destruct f0, f;
+     assert (Hneq' : n <> n0);
+     [intros Hcontra; subst; crush| apply Nat.eqb_neq in Hneq'; rewrite Hneq'; auto]].
+
+  (*new object initialization*)
+  simpl in *.
+  unfold update, t_update in H.
+  destruct (eq_dec α0 α) as [Heq|Hneq];
+    [subst; rewrite eqb_refl in H
+    |apply neq_eqb in Hneq; rewrite Hneq in H;
+     inversion H11; subst; apply (H8 α0); auto].
+  exists CDef;
+    split; [inversion H; subst; auto
+           |split;
+            [intros
+            |inversion H; subst; auto]].
+  inversion H; subst; simpl.
+  assert (Hin : fMap f = None -> ~ In f (c_flds CDef));
+    [auto|].
+  remember (fMap f) as res.
+  destruct res as [y|];
+    [
+    |contradiction Hin; auto].
+  destruct (H7 f y) as [v];
+    auto.
+  exists v; unfold compose; rewrite <- Heqres; auto.
+Qed.
+
+Lemma linking_unique :
+  forall M1 M2 M, M1 ∘ M2 ≜ M ->
+             forall M', M1 ∘ M2 ≜ M' ->
+                   M' = M.
+Proof.
+  intros M1 M2 M Hlink1 M' Hlink2;
+    inversion Hlink1; inversion Hlink2;
+      subst;
+      auto.
+Qed.
+
+Ltac link_unique_auto :=
+  match goal with
+  | [H1 : ?M1 ∘ ?M2 ≜ ?M, H2 : ?M1 ∘ ?M2 ≜ ?M' |-_] =>
+    assert (M' = M);
+    [eapply linking_unique;
+     eauto|subst M']
+  end.
+
+Ltac reduce_heap_wf_auto :=
+  match goal with
+  | [Hred : ?M ∙ ?σ1 ⤳ ?σ2 |- χ_wf ?M (fst ?σ2)] =>
+    eapply reduction_preserves_well_formed_heap; eauto
+  end.
+
+Lemma reductions_preserves_heap_wf :
+  forall M1 M2 σ1 σ2, M1 ⦂ M2 ⦿ σ1 ⤳… σ2 ->
+                 forall M, M1 ∘ M2 ≜ M ->
+                      χ_wf M (fst σ1) ->
+                      χ_wf M (fst σ2).
+Proof.
+  intros M1 M2 σ1 σ2 Hred;
+    induction Hred;
+    intros;
+    auto;
+    link_unique_auto;
+    reduce_heap_wf_auto.
+Qed.
+
+Ltac reduces_heap_wf_auto :=
+  match goal with
+  | [Hred : ?M1 ⦂ ?M2 ⦿ ?σ1 ⤳… ?σ2 |- χ_wf ?M (fst ?σ2)] =>
+    eapply reductions_preserves_heap_wf; eauto
+  end.
+
+Lemma pair_reduction_preserves_heap_wf :
+  forall M1 M2 σ1 σ2, M1 ⦂ M2 ⦿ σ1 ⤳ σ2 ->
+                 forall M, M1 ∘ M2 ≜ M ->
+                      χ_wf M (fst σ1) ->
+                      χ_wf M (fst σ2).
+Proof.
+  intros M1 M2 σ1 σ2 Hred;
+    induction Hred;
+    intros.
+  link_unique_auto.
+  reduce_heap_wf_auto.
+  reduces_heap_wf_auto.
+Qed.
+
+Ltac pair_reduce_heap_wf_auto :=
+  match goal with
+  | [Hred : ?M1 ⦂ ?M2 ⦿ ?σ1 ⤳ ?σ2 |- χ_wf ?M (fst ?σ2)] =>
+    eapply pair_reduction_preserves_heap_wf; eauto
+  end.
+
+Lemma pair_reductions_preserves_heap_wf :
+  forall M1 M2 σ1 σ2, M1 ⦂ M2 ⦿ σ1 ⤳⋆ σ2 ->
+                 forall M, M1 ∘ M2 ≜ M ->
+                      χ_wf M (fst σ1) ->
+                      χ_wf M (fst σ2).
+Proof.
+  intros M1 M2 σ1 σ2 Hred;
+    induction Hred;
+    intros;
+    auto;
+    try solve pair_reduce_heap_wf_auto.
+  eapply IHHred; eauto;
+    pair_reduce_heap_wf_auto.
+Qed.
+
+Ltac pair_reduces_heap_wf_auto :=
+  match goal with
+  | [Hred : ?M1 ⦂ ?M2 ⦿ ?σ1 ⤳⋆ ?σ2 |- χ_wf ?M (fst ?σ2)] =>
+    eapply pair_reductions_preserves_heap_wf; eauto
+  end.
+
+Lemma M_wf_ObjectDefn :
+  forall M, M_wf M ->
+       M ObjectName = Some ObjectDefn.
+Proof.
+  intros M Hwf; inversion Hwf; crush.
+Qed.
+
+Ltac obj_defn_rewrite :=
+  match goal with
+  | [H : M_wf ?M |- context[?M ObjectName]] => rewrite (M_wf_ObjectDefn M H)
+  end.
+
+Ltac empty_auto :=
+  match goal with
+  | [H : context [empty _] |- _] => unfold empty, t_empty in H; crush
+  | [|- context [empty _]] => unfold empty, t_empty; crush
+  end.
+
+Ltac update_auto :=
+  match goal with
+  | [H : (update ?a _ _) ?a = Some ?b' |- _] => unfold update, t_update in H;
+                                              subst; rewrite eqb_refl in H;
+                                              inversion H; subst
+  | [Hneq : ?a <> ?a', H : (update ?a _ _) ?a' = Some _ |- _] => unfold update, t_update in H;
+                                                              apply neq_eqb in Hneq;
+                                                              rewrite Hneq in H
+  | [Hneq : ?a' <> ?a, H : (update ?a _ _) ?a' = Some _ |- _] => unfold update, t_update in H;
+                                                              apply neq_eqb in Hneq;
+                                                              rewrite Hneq in H
+  | [H : (update ?a _ _) ?a' = Some ?b' |- _] => unfold update, t_update in H;
+                                               let Heq := fresh "Heq" in
+                                               let Hneq := fresh "Hneq" in
+                                               destruct (eq_dec a' a) as [Heq|Hneq];
+                                               [subst; rewrite eqb_refl in H;
+                                                inversion H; subst
+                                               |apply neq_eqb in Hneq;
+                                                rewrite Hneq in H]
+
+  | [H : context[(update ?a _ _) ?a]  |- _] => unfold update, t_update in H;
+                                             subst; rewrite eqb_refl in H
+  | [Hneq : ?a <> ?a', H : context[(update ?a _ _) ?a']  |- _] => unfold update, t_update in H;
+                                                               apply neq_eqb in Hneq;
+                                                               rewrite Hneq in H
+  | [Hneq : ?a' <> ?a, H : context[(update ?a _ _) ?a']  |- _] => unfold update, t_update in H;
+                                                               apply neq_eqb in Hneq;
+                                                               rewrite Hneq in H
+  | [H : context[(update ?a _ _) ?a']  |- _] => unfold update, t_update in H;
+                                              let Heq := fresh "Heq" in
+                                              let Hneq := fresh "Hneq" in
+                                              destruct (eq_dec a' a) as [Heq|Hneq];
+                                              [subst; rewrite eqb_refl in H
+                                              |apply neq_eqb in Hneq;
+                                               rewrite Hneq in H]
+                                                     
+  | [|- (update ?a _ _) ?a = Some _] => unfold update, t_update;
+                                      subst; rewrite eqb_refl
+  | [Hneq : ?a <> ?a' |- (update ?a _ _) ?a' = Some _] => unfold update, t_update;
+                                                       apply neq_eqb in Hneq;
+                                                       rewrite Hneq
+  | [Hneq : ?a' <> ?a |- (update ?a _ _) ?a' = Some _] => unfold update, t_update;
+                                                       apply neq_eqb in Hneq;
+                                                       rewrite Hneq
+  | [|- (update ?a _ _) ?a' = Some ?b'] => unfold update, t_update;
+                                         let Heq := fresh "Heq" in
+                                         let Hneq := fresh "Hneq" in
+                                         destruct (eq_dec a' a) as [Heq|Hneq];
+                                         [subst; rewrite eqb_refl
+                                         |apply neq_eqb in Hneq;
+                                          rewrite Hneq]
+                                                
+  | [|- context[(update ?a _ _) ?a]] => unfold update, t_update;
+                                      subst; rewrite eqb_refl
+  | [Hneq : ?a <> ?a' |- context[(update ?a _ _) ?a']] => unfold update, t_update;
+                                                       apply neq_eqb in Hneq;
+                                                       rewrite Hneq
+  | [Hneq : ?a' <> ?a |- context[(update ?a _ _) ?a']] => unfold update, t_update;
+                                                       apply neq_eqb in Hneq;
+                                                       rewrite Hneq
+  | [|- context[(update ?a _ _) ?a']] => unfold update, t_update;
+                                       let Heq := fresh "Heq" in
+                                       let Hneq := fresh "Hneq" in
+                                       destruct (eq_dec a' a) as [Heq|Hneq];
+                                       [subst; rewrite eqb_refl
+                                       |apply neq_eqb in Hneq;
+                                        rewrite Hneq]
+  end;
+  auto.
+
+Ltac pmap_simpl :=
+  repeat (try empty_auto;
+          try update_auto).
+
+Lemma initial_heap_wf :
+  forall σ, initial σ ->
+       forall M, M_wf M ->
+            χ_wf M (fst σ).
+Proof.
+  intros σ Hinit;
+    destruct Hinit as [α Hinit];
+    destruct Hinit as [ϕ Hinit];
+    andDestruct;
+    subst;
+    intros.
+  apply heap_wf;
+    intros.
+  simpl in H0; inversion H0; subst.
+  update_auto;
+    [exists ObjectDefn;
+     split; simpl; auto;
+     try solve [obj_defn_rewrite; auto];
+     crush
+    |empty_auto].
+Qed.
+
+Ltac initial_heap_wf_auto :=
+  match goal with
+  | [H : initial ?σ |- χ_wf ?M (fst ?σ)] => eapply initial_heap_wf; eauto
+  end.
+
+Lemma linked_wf :
+  forall M1 M2 M, M1 ∘ M2 ≜ M ->
+             M_wf M1 ->
+             M_wf M2 ->
+             M_wf M.
+Proof.
+  intros M1 M2 M Hlink Hwf1 Hwf2;
+    inversion Hlink; subst;
+      inversion Hwf1; subst;
+        inversion Hwf2; subst.
+  apply module_wf;
+    auto; intros.
+  unfold extend;
+    destruct (M1 ObjectName); auto.
+  unfold extend in H5.
+  remember (M1 C) as x;
+    destruct x; crush.
+Qed.
+
+Ltac linking_wf :=
+  match goal with
+  | [H1 : M_wf ?M1, H2 : M_wf ?M2, Hlink : ?M1 ∘ ?M2 ≜ ?M |- M_wf ?M] => eapply linked_wf; eauto
+  end.
+
+Lemma arising_heap_wf :
+  forall M1 M2 σ, arising M1 M2 σ ->
+             M_wf M1 ->
+             M_wf M2 ->
+             forall M, M1 ∘ M2 ≜ M ->
+                  χ_wf M (fst σ).
+Proof.
+  intros.
+  inversion H; subst.
+  pair_reduces_heap_wf_auto.
+  initial_heap_wf_auto.
+  linking_wf.
+Qed.
+
+Lemma exists_dom_finite :
+  forall {A B : Type} `{Eq A} (m : partial_map A B),
+    finite m ->
+    exists d, dom m d.
+Proof.
+  intros A B HeqClass m Hfinite;
+    induction Hfinite;
+    [exists nil; auto|].
+
+  destruct IHHfinite as [d Hdom].
+  destruct (excluded_middle (In a d)) as [Hin|Hnin];
+    [exists d|exists (a::d)]; auto.
+
+Qed.
+
+Lemma update_neq_empty :
+  forall {A B : Type}`{Eq A} (a : A)(b : B) m,
+    update a b m <> empty.
+Proof.
+  intros; intros Hcontra.
+  assert (Heq : update a b m a = None);
+    [rewrite Hcontra; pmap_simpl|pmap_simpl].
+  crush.
+Qed.
+
+Ltac update_empty_contra :=
+  match goal with
+  | [H : update ?a ?b ?m = empty |- _] => contradiction (update_neq_empty a b m)
+  | [H : empty = update ?a ?b ?m |- _] => symmetry in H; contradiction (update_neq_empty a b m)
+  end.
+
+Lemma dom_empty_is_nil :
+  forall {A B : Type}`{Eq A} (m : partial_map A B) d,
+    dom m d ->
+    m = empty ->
+    d = nil.
+Proof.
+  intros A B HeqClass m d H;
+    intros;
+    subst;
+    inversion H;
+    subst;
+    auto;
+    update_empty_contra.
+Qed.
+
+Lemma partial_map_dec :
+  forall {A B : Type} `{Eq A} a (m : partial_map A B), {exists b, m a = Some b} + {m a = None}.
+Proof.
+  intros.
+  destruct (m a) as [b|]; [left; exists b|]; crush.
+Qed.
+
+(*Lemma update_dom :
+  forall {A B : Type}`{Eq A} (m : partial_map A B) d,
+    dom m d ->
+    forall a b, (dom (update a b m) d) \/ (dom (update a b m) (a::d)).
+Proof.
+  intros A B HeqCl m d Hdom;
+    induction Hdom;
+    intros.
+  destruct (partial_map_dec a m) as [Hsome|Hnone];
+    [left|right].
+  apply d_map; intros; auto; [|pmap_simpl; try solve [crush]].
+  pmap_simpl;
+    [destruct Hsome as [b']
+    |pmap_simpl]; eauto.
+  exists b; auto.
+
+  apply d_map;
+    intros.
+  pmap_simpl; crush;
+    right; eapply H; eauto.
+  pmap_simpl; [exists b; auto|].
+  inversion H2; subst;
+    [apply eqb_neq in Hneq; crush
+    |crush].
+
+  apply u_con;
+    auto.
+  intro Hcontra.
+  apply H0 in Hcontra; crush.
+Qed.*)
+
+(*Lemma dom_update :
+  forall {A B : Type} `{Eq A} (m : partial_map A B) a b d,
+    dom (update a b m) d ->
+    (dom m d) \/ (exists d', dom m d' /\ (d = a :: d')).
+Proof.
+  intros;
+    inversion H0;
+    subst.
+
+  destruct (partial_map_dec a m);
+    [left|right].
+
+  apply d_map; intros; auto.
+  destruct (eq_dec a0 a) as [Heq|Hneq];
+    [subst; apply (H1 a b);
+     pmap_simpl;
+     auto
+    |eapply H1; pmap_simpl; eauto].
+  destruct (eq_dec a0 a) as [Heq|Hneq];
+    [subst;
+     pmap_simpl;
+     auto
+    |eapply H2 in H4; pmap_simpl; auto].
+
+  destruct d as [|a' d'];
+    [assert (Hin : In a nil);
+     [apply (H1 a b); eauto; pmap_simpl; auto|crush]
+    |exists d'; split].
+  apply d_map;
+    intros;
+    auto.
+
+  destruct (eq_dec a a0) as [Heq|Hneq];
+    [subst; crush|].
+  assert (Hin : In a0 (a'::d'));
+    [apply H1 with (b0:=b0);
+     pmap_simpl; crush
+    |inversion Hin; subst; auto].
+
+Qed.*)
+    
+
+Lemma zip_length_exists :
+  forall {A B : Type} (l1 : list A) (l2 : list B),
+    length l1 = length l2 ->
+    exists z, zip l1 l2 z.
+Proof.
+  intros A B l1;
+    induction l1 as [|a l];
+    intros.
+  exists nil;
+    destruct l2;
+    [auto|inversion H].
+  destruct l2 as [|b l'];
+    [inversion H
+    |simpl in H;
+     destruct (IHl l') as [z Hzip];
+     auto].
+  exists ((a,b)::z); auto.
+Qed.
+
+Lemma fresh_in_empty :
+  forall {A : Type} x, @fresh_in_map A x empty.
+Proof.
+  unfold fresh_in_map;
+    intros.
+  pmap_simpl.
+Qed.
+
+Hint Resolve fresh_in_empty.
+
+Lemma map_implies_in_dom :
+  forall {A B : Type} `{Eq A} (m : partial_map A B) d,
+    dom m d ->
+    forall a b, m a = Some b ->
+           In a d.
+Proof.
+  intros A B HeqClass m d Hdom;
+    induction Hdom;
+    intros;
+    try solve [pmap_simpl; crush; eauto].
+Qed.
+
+Lemma in_dom_implies_in_map :
+  forall {A B : Type} `{Eq A} (m : partial_map A B) d,
+    dom m d ->
+    forall a, In a d ->
+    exists b, m a = Some b.
+Proof.
+  intros A B HeqClass m d Hdom;
+    induction Hdom;
+    intros;
+    pmap_simpl;
+    try solve [eexists; eauto].
+
+  inversion H0;
+    subst;
+    [apply eqb_neq in Hneq;
+     crush
+    |eapply IHHdom; eauto].
+
+Qed.
+
+Lemma fresh_in_map_not_in_dom :
+  forall {A : Type} (m : partial_map var A) d,
+    dom m d ->
+    forall x, fresh_in_map x m <-> ~ In x d.
+Proof.
+  intros A m d Hdom;
+    induction Hdom;
+    intros;
+    split;
+    auto;
+    unfold fresh_in_map;
+    intros;
+    auto.
+
+  apply IHHdom;
+    unfold fresh_in_map;
+    intros;
+    destruct (eq_dec a y) as [Heq|Hneq];
+    [subst; apply (H0 y b)
+    |apply (H0 y a0)];
+    pmap_simpl; crush.
+
+  intros Hcontra;
+    subst;
+    pmap_simpl;
+    apply map_implies_in_dom
+    with (a1:=y)(b0:=a0)
+    in Hdom;
+    crush.
+
+  intros Hcontra;
+    inversion Hcontra;
+    subst;
+    [destruct (H0 x b); pmap_simpl; auto|];
+    destruct (in_dom_implies_in_map m d) with (a:=x);
+    auto;
+    destruct (eq_dec x a) as [Heq|Hneq];
+    [subst;
+     contradiction (H0 a b);
+     auto; pmap_simpl
+    |contradiction (H0 x x0);
+     auto; pmap_simpl].
+
+  intros Hcontra;
+    subst.
+  pmap_simpl;
+    [contradiction H0;
+     crush
+    |].
+  assert (Hnin : ~ In y d);
+    [intros Hcontra;
+     crush
+    |apply <- IHHdom in Hnin].
+  unfold fresh_in_map in Hnin;
+    apply Hnin in H1;
+    crush.
+Qed.
+
+Inductive lt_map {A : Type} : nat -> partial_map var A -> Prop :=
+| lt_empty : lt_map 0 empty
+| lt_update1 : forall n b m n', lt_map n' m ->
+                           n < n' ->
+                           lt_map n' (update (bind n) b m)
+| lt_update2 : forall n b m n', lt_map n' m ->
+                           n' <= n ->
+                           lt_map (S n) (update (bind n) b m).
+
+Hint Constructors lt_map.
+
+Lemma exists_limit_for_finite_map :
+  forall {A : Type} (m : partial_map var A),
+    finite m ->
+    exists n, lt_map n m.
+Proof.
+  intros A m Hfinite;
+    induction Hfinite;
+    [exists 0; auto|destruct IHHfinite as [n]].
+  
+  destruct a as [n'].
+  destruct (le_lt_dec n n') as [Hle|Hlt];
+    [exists (S n'); eapply lt_update2|exists n; apply lt_update1]; eauto.
+Qed.
+
+Lemma lt_map_implies_var_lt :
+  forall {A : Type} n (m : partial_map var A),
+    lt_map n m ->
+    forall n' b, m (bind n') = Some b ->
+            n' < n.
+Proof.
+  intros A n m Hlt;
+    induction Hlt;
+    intros;
+    pmap_simpl.
+  destruct (eq_dec n'0 n);
+    [subst|];
+    pmap_simpl.
+  unfold update, t_update in H0;
+    rewrite neq_eqb in H0; [eauto|crush].
+  destruct (eq_dec n'0 n);
+    [subst|];
+    pmap_simpl.
+  unfold update, t_update in H0;
+    rewrite neq_eqb in H0; [eauto|crush].
+  apply IHHlt in H0; crush.
+Qed.
+
+Lemma lt_fresh_in_map :
+  forall {A : Type} n (m : partial_map var A),
+    lt_map n m -> forall n', n <= n' -> fresh_in_map (bind n') m.
+Proof.
+  intros A n m Hlt;
+    induction Hlt;
+    auto;
+    unfold fresh_in_map in *;    
+    intros;
+    pmap_simpl;
+    try solve [crush];
+    eauto.
+
+  destruct y as [n''].
+  eapply lt_map_implies_var_lt in Hlt;
+    eauto;
+    crush.
+Qed.
+
+Lemma fresh_var_finite :
+  forall {A : Type} (m : partial_map var A),
+    finite m ->
+    exists x, fresh_in_map x m.
+Proof.
+  intros;
+    destruct (exists_limit_for_finite_map m) as [n];
+    auto;
+    exists (bind n);
+    eapply lt_fresh_in_map;
+    eauto.
+Qed.
+
+Lemma fresh_var_finite2 :
+  forall {A : Type} (m1 : partial_map var A),
+    finite m1 ->
+    forall (m2 : partial_map var A), finite m2 ->
+                                exists x, fresh_in_map x m1 /\
+                                     fresh_in_map x m2.
+Proof.
+  intros.
+  destruct (exists_limit_for_finite_map m1) as [n1];
+    destruct (exists_limit_for_finite_map m2) as [n2];
+    auto.
+  destruct (le_lt_dec n1 n2) as [Hle|Hlt];
+    [exists (bind n2)|exists (bind n1)];
+    split;
+    eapply lt_fresh_in_map;
+    eauto;
+    crush.
+Qed.
+
+Inductive lt_var : nat -> var -> Prop :=
+| lt_bind : forall n n', n' < n ->
+                    lt_var n (bind n').
+
+Hint Constructors lt_var.
+
+Lemma exists_limit_var :
+  forall x, exists n, lt_var n x.
+Proof.
+  intros x;
+    destruct x as [n'];
+    exists (S n');
+    crush.
+Qed.
+
+Lemma exists_limit_for_list :
+  forall l, exists n, forall x, In x l ->
+                 lt_var n x.
+Proof.
+  intros l;
+    induction l as [|x l'];
+    [exists 0; crush|destruct x as [n']].
+  destruct IHl' as [n Hltx].
+  destruct (le_lt_dec n n') as [Hle|Hlt];
+    [exists (S n')|exists n];
+    intros.
+  inversion H; subst; crush.
+  apply Hltx in H0.
+  inversion H0; subst; crush.
+  crush.
+Qed.
+
+Lemma fresh_var_finite3 :
+  forall {A : Type} (m1 : partial_map var A),
+    finite m1 ->
+    forall (m2 : partial_map var A), finite m2 ->
+                                forall d, exists x, fresh_in_map x m1 /\
+                                          fresh_in_map x m2 /\
+                                          ~ In x d.
+Proof.
+  intros.
+  destruct (exists_limit_for_finite_map m1) as [n1];
+    destruct (exists_limit_for_finite_map m2) as [n2];
+    destruct (exists_limit_for_list d) as [n3];
+    auto.
+  destruct (le_lt_dec n1 n2) as [Hle1|Hlt1].
+  destruct (le_lt_dec n1 n3) as [Hle2|Hlt2].
+  
+  destruct (le_lt_dec n3 n2) as [Hle3|Hlt3];
+
+    try solve [exists (bind n2); split; [|split];
+                 try solve [eapply lt_fresh_in_map; eauto; crush];
+                 intro Hcontra;
+                 apply H3 in Hcontra;
+                 inversion Hcontra; crush];
+
+    try solve [exists (bind n3); split; [|split];
+                 try solve [eapply lt_fresh_in_map; eauto; crush];
+                 intro Hcontra;
+                 apply H3 in Hcontra;
+                 inversion Hcontra; crush].
+  
+  destruct (le_lt_dec n3 n2) as [Hle3|Hlt3];
+
+    try solve [exists (bind n2); split; [|split];
+                 try solve [eapply lt_fresh_in_map; eauto; crush];
+                 intro Hcontra;
+                 apply H3 in Hcontra;
+                 inversion Hcontra; crush];
+
+    try solve [exists (bind n3); split; [|split];
+                 try solve [eapply lt_fresh_in_map; eauto; crush];
+                 intro Hcontra;
+                 apply H3 in Hcontra;
+                 inversion Hcontra; crush].
+  
+  destruct (le_lt_dec n1 n3) as [Hle2|Hlt2];
+
+    try solve [exists (bind n1); split; [|split];
+                 try solve [eapply lt_fresh_in_map; eauto; crush];
+                 intro Hcontra;
+                 apply H3 in Hcontra;
+                 inversion Hcontra; crush];
+
+    try solve [exists (bind n3); split; [|split];
+                 try solve [eapply lt_fresh_in_map; eauto; crush];
+                 intro Hcontra;
+                 apply H3 in Hcontra;
+                 inversion Hcontra; crush].
+Qed.
+
+Lemma dom_implies_finite :
+  forall {A : Type} (m : partial_map var A) d,
+    dom m d ->
+    finite m.
+Proof.
+  intros A m d Hdom;
+    induction Hdom;
+    crush.
+Qed.
+
+(** TODO: *)
+Parameter fresh_var_list_finite :
+  forall {A : Type} (m1 : partial_map var A) (d : list var),
+    dom m1 d ->
+    forall (m2 : partial_map var A) s,
+      finite m2 ->
+      exists d' D,
+        (forall z, In z d' -> fresh_in_map z m1) /\
+        (forall z, In z d' -> fresh_in_map z m2) /\
+        (forall z, In z d' -> ~ in_stmt z s) /\
+        unique d' /\
+        zip d' d D.
+
+Ltac finite_auto :=
+  repeat match goal with
+         | [H : context[finite_σ _] |- _] => unfold finite_σ in H
+         | [H : context[finite_ψ _] |- _] => unfold finite_ψ in H
+         | [H : context[finite_ϕ _] |- _] => unfold finite_ϕ in H
+         | [|- context[finite_σ _]] => unfold finite_σ
+         | [|- context[finite_ψ _]] => unfold finite_ψ
+         | [|- context[finite_ϕ _]] => unfold finite_ϕ
+         end.
+
+Ltac not_stuck_auto :=
+  repeat match goal with
+         | [H : context[not_stuck_σ _] |- _] => unfold not_stuck_σ in H
+         | [H : context[not_stuck_ϕ _] |- _] => unfold not_stuck_ϕ in H
+         | [|- context[not_stuck_σ _]] => unfold not_stuck_σ
+         | [|- context[not_stuck_ϕ _]] => unfold not_stuck_ϕ
+         end.
+
+Ltac waiting_auto :=
+  repeat match goal with
+         | [H : context[waiting_σ _] |- _] => unfold waiting_σ in H
+         | [H : context[waiting_ψ _] |- _] => unfold waiting_ψ in H
+         | [H : context[waiting_ϕ _] |- _] => unfold waiting_ϕ in H
+         | [|- context[waiting_σ _]] => unfold waiting_σ
+         | [|- context[waiting_ψ _]] => unfold waiting_ψ
+         | [|- context[waiting_ϕ _]] => unfold waiting_ϕ
+         end.
+
+Lemma dom_unique :
+  forall {A B : Type} `{Eq A} (m : partial_map A B) d,
+    dom m d ->
+    unique d.
+Proof.
+  intros A B HeqClass m d Hdom;
+    induction Hdom;
+    auto.
+Qed.
+
+Lemma adaptation_exists :
+  forall σ1 σ2, finite_σ σ1 ->
+           finite_σ σ2 ->
+           not_stuck_σ σ2 ->
+           forall χ1 ϕ1 ψ1
+             χ2 ϕ2 ψ2,
+             σ1 = (χ1, ϕ1::ψ1) ->
+             σ2 = (χ2, ϕ2::ψ2) ->
+             exists σ, σ1 ◁ σ2 ≜ σ.
+Proof.
+  intros.
+  
+  unfold not_stuck_σ, not_stuck_ϕ in H1.
+  destruct H1 as [ϕ' Hnstuck];
+    destruct Hnstuck as [ψ' Hnstuck];
+    andDestruct.
+  inversion Hb; subst; simpl in *;
+    inversion Ha; subst.
+  
+  remember (vMap ϕ1) as β1.
+  destruct (exists_dom_finite β1) as [zs]; auto;
+    [subst; finite_auto; 
+     apply H; crush|].
+  remember (vMap ϕ') as β2.
+  
+  destruct (fresh_var_list_finite β1 zs H1 β2 s) as [zs' Hfresh];
+    [finite_auto; crush
+    |destruct Hfresh as [D Hfresh];
+     andDestruct].
+
+  (exists (χ2, (frm (updates D β1 β2) (c_stmt (rename_s s D)))::ψ')).
+  apply a_adapt
+    with
+      (ϕ:=ϕ1)(ϕ':=ϕ')(contn:=contn ϕ1)
+      (β:=β1)(β':=β2)(β'':=updates D β1 β2)
+      (zs:=zs)(zs':=zs')(s:=s)
+      (s':=rename_s s D)(Zs:=D);
+    auto;
+    try solve [crush].
+  destruct ϕ1;
+    f_equal;
+    auto.
+  destruct ϕ';
+    f_equal;
+    auto.
+
+  eapply dom_unique; eauto.
+  
+Qed.
+
+Inductive finite_normal_form {A B : Type} `{Eq A} : partial_map A B -> Prop :=
+| norm_empty : finite_normal_form empty
+| norm_update : forall a b m, finite_normal_form m ->
+                         m a = None ->
+                         finite_normal_form (update a b m).
+
+Hint Constructors finite_normal_form.
+
+Lemma compose_normal_form :
+  forall {A B : Type}`{Eq A}`{Eq B} (m1 : partial_map A B),
+    finite_normal_form m1 ->
+    forall {C : Type} (m2 : partial_map B C),
+    exists m3, finite_normal_form m3 /\ m3 = compose m1 m2.
+Proof.
+  intros A B HeqClassA HeqClassB m1 Hnorm;
+    induction Hnorm;
+    intros;
+    auto.
+
+  exists empty; auto.
+
+  destruct (IHHnorm C m2) as [m3 IH];
+    destruct IH as [IH1 IH2].
+  destruct (partial_map_dec b m2)
+    as [HSome|HNone];
+    [destruct HSome as [c HSome]|].
+  unfold compose;
+    exists (update a c m3);
+    split;
+    [apply norm_update;
+     subst m3;
+     unfold compose; [auto|crush]|].
+    apply functional_extensionality;
+    intros a';
+    pmap_simpl;
+    crush.
+  exists m3;
+    split;
+    auto.
+  subst; unfold compose; auto.
+  apply functional_extensionality;
+    intros c;
+    pmap_simpl;
+    crush.
+Qed.
+
+Lemma update_finite_normal_form :
+  forall {A B : Type} `{Eq A} (m : partial_map A B),
+    finite_normal_form m ->
+    forall a b, exists m', finite_normal_form m' /\ m' = (update a b m).
+Proof.
+  intros A B HeqClass m Hfinite;
+    induction Hfinite;
+    intros;
+    [exists (update a b empty); auto|].
+
+  destruct (IHHfinite a0 b0) as [m' Hnorm];
+    destruct Hnorm as [Hnorm Heqm'].
+
+  destruct (eq_dec a0 a) as [Heq|Hneq];
+    [subst a0
+    |].
+
+  exists m'; split; auto;
+    apply functional_extensionality;
+    intros a';
+    subst;
+    pmap_simpl.
+
+  exists (update a b m');
+    split.
+
+  destruct (partial_map_dec a m') as [HSome|HNone];
+    [destruct HSome as [b' HSome]; subst; pmap_simpl; crush
+    |apply norm_update; auto].
+
+  apply functional_extensionality; intros a'; pmap_simpl; subst.
+  rewrite neq_eqb; auto.
+  destruct (eq_dec a' a0) as [Heqa'|Hneqa'];
+    [subst; pmap_simpl|pmap_simpl].
+Qed.
+
+Lemma finite_exists_normal_form :
+  forall {A B : Type} `{Eq A} (m : partial_map A B),
+    finite m ->
+    exists m', finite_normal_form m' /\ m' = m.
+Proof.
+  intros A B HeqClass m Hfinite;
+    induction Hfinite;
+    [exists empty; auto|].
+
+  apply update_finite_normal_form; crush.
+Qed.
+
+Lemma finite_normal_form_implies_finite :
+  forall {A B : Type} `{Eq A} (m : partial_map A B),
+    finite_normal_form m ->
+    finite m.
+Proof.
+  intros A B HeqClass m Hnorm;
+    induction Hnorm;
+    auto.
+Qed.
+
+Lemma finite_implies_normal_form :
+  forall {A B : Type} `{Eq A} (m : partial_map A B),
+    finite m ->
+    finite_normal_form m.
+Proof.
+  intros.
+  destruct (finite_exists_normal_form m);
+    andDestruct;
+    subst;
+    auto.
+Qed.
+
+Hint Resolve finite_implies_normal_form finite_exists_normal_form finite_normal_form_implies_finite
+     compose_normal_form.
+
+Lemma finite_map_composition :
+  forall {A B : Type}`{Eq A}`{Eq B} (m1 : partial_map A B),
+    finite m1 ->
+    forall {C : Type} (m2 : partial_map B C),
+      finite (compose m1 m2).
+Proof.
+  intros.
+  destruct (compose_normal_form m1 (finite_implies_normal_form m1 H1) m2); eauto.
+  andDestruct; subst.
+  apply finite_normal_form_implies_finite; auto.
+Qed.
+
+Ltac peek_pop_simpl :=
+  match goal with
+  | [H : peek ?ψ = Some ?ϕ |- _] => let ϕ' := fresh "ϕ'" in
+                                  let ψ' := fresh "ψ'" in
+                                  destruct ψ as [|ϕ' ψ'];
+                                  simpl in H;
+                                  inversion H;
+                                  subst
+  | [H : pop ?ψ = Some ?ψ' |- _] => let ϕ' := fresh "ϕ'" in
+                                  let ψ'' := fresh "ψ''" in
+                                  destruct ψ as [|ϕ' ψ'];
+                                  simpl in H;
+                                  inversion H;
+                                  subst
+  end.
+
+Lemma reduction_preserves_config_finiteness :
+  forall M σ1 σ2, M ∙ σ1 ⤳ σ2 ->
+             finite_σ σ1 ->
+             finite_σ σ2.
+Proof.
+  intros M σ1 σ2 Hred;
+    induction Hred;
+    intros;
+    subst;
+    finite_auto;
+    simpl in *;
+    intros;
+    auto.
+
+  destruct H as [Ha|Ha];
+    [|destruct Ha as [Ha|Ha]];
+    subst;
+    simpl;
+    [apply fin_update;
+     apply finite_map_composition;
+     auto
+    | |];
+    peek_pop_simpl;
+    crush.
+
+  peek_pop_simpl;
+  unfold update_ψ_map, update_ϕ_map in H0;
+    inversion H0;
+    subst;
+    [simpl; apply fin_update|];
+    apply H9; crush.
+
+  destruct H; [subst; simpl|]; eauto.
+
+  peek_pop_simpl.
+  destruct H; crush.
+
+  unfold update_ϕ_contn, update_ϕ_map in H; simpl in H;
+    destruct H; crush.
+
+  peek_pop_simpl.
+  unfold update_ϕ_contn, update_ϕ_map in H; simpl in H;
+    destruct H; crush.
+  apply fin_update.
+  peek_pop_simpl.
+  simpl in H1;
+    inversion H1; subst; crush.
+
+  peek_pop_simpl.
+  apply H8; crush.
+Qed.
+
+Hint Resolve reduction_preserves_config_finiteness.
+
+Lemma reductions_preserves_config_finiteness :
+  forall M1 M2 σ1 σ2, M1 ⦂ M2 ⦿ σ1 ⤳… σ2 ->
+                 finite_σ σ1 ->
+                 finite_σ σ2.
+Proof.
+  intros M1 M2 σ1 σ2 Hred;
+    induction Hred;
+    intros;
+    crush;
+    eauto.
+Qed.
+
+Hint Resolve reductions_preserves_config_finiteness.
+
+Lemma pair_reduction_preserves_config_finiteness :
+  forall M1 M2 σ1 σ2, M1 ⦂ M2 ⦿ σ1 ⤳ σ2 ->
+                 finite_σ σ1 ->
+                 finite_σ σ2.
+Proof.
+  intros M1 M2 σ1 σ2 Hred;
+    inversion Hred;
+    subst;
+    intros;
+    crush;
+    eauto.
+Qed.
+
+Hint Resolve pair_reduction_preserves_config_finiteness.
+
+Lemma pair_reductions_preserves_config_finiteness :
+  forall M1 M2 σ1 σ2, M1 ⦂ M2 ⦿ σ1 ⤳⋆ σ2 ->
+                 finite_σ σ1 ->
+                 finite_σ σ2.
+Proof.
+  intros M1 M2 σ1 σ2 Hred;
+    induction Hred;
+    subst;
+    intros;
+    eauto.
+Qed.
+
+Hint Resolve pair_reductions_preserves_config_finiteness.
+
+Lemma reduction_preserves_config_not_stuck :
+  forall M σ1 σ2, M ∙ σ1 ⤳ σ2 ->
+             not_stuck_σ σ1 ->
+             not_stuck_σ σ2.
+Proof.
+  intros M σ1 σ2 Hred;
+    induction Hred;
+    intros;
+    unfold not_stuck_σ in *;
+    simpl in *;
+    try solve [eexists; crush; eauto].
+
+  exists ϕ'', (ϕ'::ψ'); split;
+    unfold not_stuck_ϕ;
+    subst;
+    simpl in *;
+    eauto.
+
+  subst σ'; simpl;
+    exists ϕ', ψ;
+    split;
+    auto;
+    subst ϕ';
+    unfold not_stuck_ϕ;
+    simpl;
+    auto.
+
+  subst σ'; simpl;
+    exists ϕ', ψ';
+    split;
+    auto;
+    subst ϕ';
+    unfold not_stuck_ϕ;
+    simpl;
+    auto.
+
+  exists ϕ'', ψ;
+    split;
+    auto;
+    subst ϕ'';
+    unfold not_stuck_ϕ;
+    simpl;
+    auto.
+
+  exists ϕ'', ψ'';
+    split;
+    auto;
+    subst ϕ'';
+    unfold not_stuck_ϕ;
+    simpl;
+    auto.
+Qed.
+
+Hint Resolve reduction_preserves_config_not_stuck.
+
+Lemma reductions_preserves_config_not_stuck :
+  forall M1 M2 σ1 σ2, M1 ⦂ M2 ⦿ σ1 ⤳… σ2 ->
+                 not_stuck_σ σ1 ->
+                 not_stuck_σ σ2.
+Proof.
+  intros M1 M2 σ1 σ2 Hred;
+    induction Hred;
+    intros;
+    eauto.
+Qed.
+
+Hint Resolve reductions_preserves_config_not_stuck.
+
+Lemma pair_reduction_preserves_config_not_stuck :
+  forall M1 M2 σ1 σ2, M1 ⦂ M2 ⦿ σ1 ⤳ σ2 ->
+                 not_stuck_σ σ1 ->
+                 not_stuck_σ σ2.
+Proof.
+  intros M1 M2 σ1 σ2 Hred;
+    induction Hred;
+    intros;
+    eauto.
+Qed.
+
+Hint Resolve pair_reduction_preserves_config_not_stuck.
+
+Lemma pair_reductions_preserves_config_not_stuck :
+  forall M1 M2 σ1 σ2, M1 ⦂ M2 ⦿ σ1 ⤳⋆ σ2 ->
+                 not_stuck_σ σ1 ->
+                 not_stuck_σ σ2.
+Proof.
+  intros M1 M2 σ1 σ2 Hred;
+    induction Hred;
+    intros;
+    eauto.
+Qed.
+
+Hint Resolve pair_reductions_preserves_config_not_stuck.
+
+Lemma reduction_preserves_config_waiting :
+  forall M σ1 σ2, M ∙ σ1 ⤳ σ2 ->
+             waiting_σ σ1 ->
+             waiting_σ σ2.
+Proof.
+  intros M σ1 σ2 Hred;
+    induction Hred;
+    intros;
+    unfold waiting_σ in *;
+    simpl in *;
+    try solve [eexists; crush; eauto].
+
+  exists ϕ'', (ϕ'::ψ'); split;
+    unfold waiting_ψ, waiting_ϕ in *;
+    subst;
+    intros;
+    eauto;
+    crush.
+
+  exists ϕ'', ψ;
+    split;
+    auto;
+    subst ϕ'';
+    unfold waiting_ψ, waiting_ϕ in *;
+    simpl;
+    auto;
+    crush.
+
+  exists ϕ'', ψ'';
+    split;
+    auto;
+    subst ϕ'';
+    unfold waiting_ψ, waiting_ϕ in *;
+    simpl;
+    auto;
+    crush.
+  peek_pop_simpl; crush.
+Qed.
+
+Hint Resolve reduction_preserves_config_waiting.
+
+Lemma reductions_preserves_config_waiting :
+  forall M1 M2 σ1 σ2, M1 ⦂ M2 ⦿ σ1 ⤳… σ2 ->
+                 waiting_σ σ1 ->
+                 waiting_σ σ2.
+Proof.
+  intros M1 M2 σ1 σ2 Hred;
+    induction Hred;
+    intros;
+    eauto.
+Qed.
+
+Hint Resolve reductions_preserves_config_waiting.
+
+Lemma pair_reduction_preserves_config_waiting :
+  forall M1 M2 σ1 σ2, M1 ⦂ M2 ⦿ σ1 ⤳ σ2 ->
+                 waiting_σ σ1 ->
+                 waiting_σ σ2.
+Proof.
+  intros M1 M2 σ1 σ2 Hred;
+    induction Hred;
+    intros;
+    eauto.
+Qed.
+
+Hint Resolve pair_reduction_preserves_config_waiting.
+
+Lemma pair_reductions_preserves_config_waiting :
+  forall M1 M2 σ1 σ2, M1 ⦂ M2 ⦿ σ1 ⤳⋆ σ2 ->
+                 waiting_σ σ1 ->
+                 waiting_σ σ2.
+Proof.
+  intros M1 M2 σ1 σ2 Hred;
+    induction Hred;
+    intros;
+    eauto.
+Qed.
+
+Hint Resolve pair_reductions_preserves_config_waiting.
+
+Lemma reduction_preserves_config_wf :
+  forall M σ1 σ2, M ∙ σ1 ⤳ σ2 ->
+             σ_wf σ1 ->
+             σ_wf σ2.
+Proof.
+  intros M σ1 σ2 Hred Hwf;
+    inversion Hwf; eauto.
+Qed.
+
+Hint Resolve reduction_preserves_config_wf.
+
+Lemma reductions_preserves_config_wf :
+  forall M1 M2 σ1 σ2, M1 ⦂ M2 ⦿ σ1 ⤳… σ2 ->
+             σ_wf σ1 ->
+             σ_wf σ2.
+Proof.
+  intros M1 M2 σ1 σ2 Hred Hwf;
+    inversion Hwf;
+    subst;
+    eauto.
+Qed.
+
+Hint Resolve reductions_preserves_config_wf.
+
+Lemma pair_reduction_preserves_config_wf :
+  forall M1 M2 σ1 σ2, M1 ⦂ M2 ⦿ σ1 ⤳ σ2 ->
+                 σ_wf σ1 ->
+                 σ_wf σ2.
+Proof.
+  intros M1 M2 σ1 σ2 Hred Hwf;
+    inversion Hwf;
+    eauto.
+Qed.
+
+Hint Resolve pair_reduction_preserves_config_wf.
+
+Lemma pair_reductions_preserves_config_wf :
+  forall M1 M2 σ1 σ2, M1 ⦂ M2 ⦿ σ1 ⤳⋆ σ2 ->
+                 σ_wf σ1 ->
+                 σ_wf σ2.
+Proof.
+  intros M1 M2 σ1 σ2 Hred Hwf;
+    inversion Hwf;
+    eauto.
+Qed.
+
+Hint Resolve pair_reductions_preserves_config_wf.
+
+Lemma config_head_wf :
+  forall σ, σ_wf σ ->
+       forall χ ϕ ψ, σ = (χ, ϕ::ψ) ->
+                σ_wf (χ, ϕ::nil).
+Proof.
+  intros;
+    subst.
+  inversion H;
+    subst;
+    apply config_wf;
+    finite_auto; not_stuck_auto; waiting_auto;
+      try solve [crush].
+  exists ϕ, nil; split; auto; crush.
+  exists ϕ, nil; split; auto; crush.
+Qed.
+
+Hint Resolve config_head_wf.
+
+Lemma config_wf_decompose :
+  forall σ, σ_wf σ ->
+       exists χ ϕ ψ, σ = (χ, ϕ::ψ).
+Proof.
+  intros σ Hwf;
+    inversion Hwf;
+    subst;
+    not_stuck_auto.
+  destruct H0 as [ϕ Hns];
+    destruct Hns as [ψ];
+    andDestruct.
+  exists (fst σ), ϕ, ψ; destruct σ; crush.
+Qed.
+
+Theorem eval_unique :
+  forall M σ e v1, M ∙ σ ⊢ e ↪ v1 ->
+              forall v2, M ∙ σ ⊢ e ↪ v2 ->
+                    v2 = v1.
+Proof.
+  intros M σ e v1 Heval;
+    induction Heval;
+    intros;
+    try solve [inversion H; subst; [eauto| eauto];
+               apply IHHeval1 in H6; inversion H6].
+
+  (** Case 1: eval v *)
+  inversion H; eauto.
+
+  (** Case 2: eval x *)
+  inversion H0; subst; crush.
+
+  (** Case 3: e.f *)
+  inversion H1; subst; crush.
+  apply IHHeval in H4; subst; crush.
+
+  (** Case 4: e0.g(e) *)
+  inversion H2; subst.
+  apply IHHeval1 in H6; inversion H6; subst.
+  rewrite H7 in H; inversion H; subst.
+  rewrite H8 in H0; inversion H0; subst.
+  rewrite H11 in H1; inversion H1; subst.
+  apply IHHeval2 in H13; subst.
+  apply IHHeval3 in H14; subst; auto.
+
+  (** Case 5: e1 = e2 *) 
+  inversion H; subst; eauto.
+  apply IHHeval1 in H2; apply IHHeval2 in H5; subst; crush.
+
+  (** Case 6: e1 ≠ e2 *)
+  inversion H0; subst; eauto.
+  apply IHHeval1 in H5; apply IHHeval2 in H7; subst; crush.
+Qed.
+
+Hint Rewrite eval_unique.
+
+Ltac eval_rewrite :=
+  repeat match goal with
+         | [H1 : ?M ∙ ?σ ⊢ ?e ↪ ?v1, H2 : ?M ∙ ?σ ⊢ ?e ↪ ?v2 |- _] =>
+           eapply (eval_unique M σ e v1 H1) in H2;
+           eauto;
+           subst
+         end.
+
+Lemma unique_interpretation_x :
+  forall x σ v1, ⌊ x ⌋ σ ≜ v1 ->
+            forall v2, ⌊ x ⌋ σ ≜ v2 ->
+                  v2 = v1.
+Proof.
+  intros x σ v1 Hint1 v2 Hint2;
+    inversion Hint1;
+    inversion Hint2;
+    subst.
+  rewrite H6 in H0;
+    inversion H0;
+    subst.
+  rewrite H7 in H1;
+    inversion H1;
+    subst;
+    auto.
+Qed.
+
+Lemma unique_interpretation_Σ :
+  forall Σ σ αs1, ⌊ Σ ⌋ σ ≜′ αs1 ->
+            forall αs2, ⌊ Σ ⌋ σ ≜′ αs2 ->
+                   αs2 = αs1.
+Proof.
+  intros x σ α1 Hint1;
+    induction Hint1;
+    intros αs2 Hint2;
+    inversion Hint2;
+    subst;
+    auto.
+  eapply (unique_interpretation_x x σ α) in H2;
+    subst;
+    eauto.
+  rewrite (IHHint1 αs0); auto.
+Qed.
+
+Ltac interpretation_rewrite :=
+  repeat match goal with
+         | [H1 : ⌊ ?x ⌋ ?σ ≜ ?v1, H2 : ⌊ ?x ⌋ ?σ ≜ ?v2 |- _] =>
+           eapply (unique_interpretation_x x σ v1 H1) in H2;
+           eauto;
+           subst
+         | [H1 : ⌊ ?Σ ⌋ ?σ ≜′ ?αs1, H2 : ⌊ ?Σ ⌋ ?σ ≜′ ?αs2 |- _] =>
+           eapply (unique_interpretation_Σ Σ σ αs1 H1) in H2;
+           eauto;
+           subst
+         end.
+
+Lemma wf_σ_explode :
+  forall σ, σ_wf σ ->
+       exists χ ψ ϕ, σ = (χ, ϕ::ψ) /\
+                finite (vMap ϕ) /\
+                (forall ϕ', In ϕ' ψ ->
+                       finite (vMap ϕ')) /\
+                not_stuck (contn ϕ) /\
+                (forall ϕ', In ϕ' ψ ->
+                       waiting (contn ϕ')).
+Proof.
+  intros σ Hwf;
+    inversion Hwf;
+    subst;
+    destruct σ as [χ ψ];
+    finite_auto;
+    not_stuck_auto;
+    waiting_auto;
+    crush;
+    eexists;
+    eexists;
+    eexists;
+    split;
+    eauto;
+    split;
+    eauto.
+Qed.
+
+Ltac config_wf_destruct :=
+  match goal with
+  | [H : σ_wf ?σ |-_] =>
+    apply wf_σ_explode in H;
+    let χ := fresh "χ" in
+    let ψ := fresh "ψ" in
+    let ϕ := fresh "ϕ" in
+    let Hwf := fresh "Hwf" in
+    destruct H as [χ Hwf];
+    destruct Hwf as [ψ Hwf];
+    destruct Hwf as [ϕ Hwf];
+    let Htmp := fresh "Htmp" in
+    let Hfiniteϕ := fresh "Hfiniteϕ" in
+    let Hfiniteψ := fresh "Hfiniteψ" in
+    let Hnot_stuck := fresh "Hnot_stuck" in
+    let Hwaiting := fresh "Hwaiting" in
+    destruct Hwf as [Htmp Hwf];
+    destruct Hwf as [Hfiniteϕ Hwf];
+    destruct Hwf as [Hfiniteψ Hwf];
+    destruct Hwf as [Hnot_stuck Hwaiting];
+    subst σ
+  end.
+
+Definition one_to_one {A B : Type} `{Eq A} (m : partial_map A B) : Prop :=
+  forall a1 a2 b, m a1 = Some b ->
+             m a2 = Some b ->
+             a1 = a2.
+
+(** TODO: *)
+Parameter function_neq_exists_neq_mapping  :
+    forall {A B : Type} (f1 f2 : A -> B),
+      f1 <> f2 ->
+      exists a, f1 a <> f2 a.
+
+(*Lemma compose_equality :
+  forall {A B C : Type} `{Eq A} `{Eq B} (m1 m2 : partial_map A B) (m : partial_map B C),
+    compose m1 m = compose m2 m ->
+    one_to_one m ->
+    m1 = m2.
+Proof.
+  intros.
+  destruct (excluded_middle (m1 = m2));
+    auto.
+  destruct (function_neq_exists_neq_mapping m1 m2) as [a Ha];
+    auto.
+  apply equal_f with (x:=a) in H1.
+  unfold compose in H1.
+  destruct (m1 a) as [b1|];
+    destruct (m2 a) as [b2|].
+
+  remember (m b1) as res1;
+    remember (m b2) as res2;
+    symmetry in Heqres1;
+    symmetry in Heqres2.
+  destruct (res1) as [c1|];
+    destruct (res2) as [c2|];
+    try solve [inversion H1].
+  inversion H1; subst c1.
+  apply (H2 b1 b2) in Heqres1; crush.
+  
+  
+  contradiction H3.
+  
+  apply functional_extensionality;
+    intros a.
+  
+Qed.*)
+
+(** This theorem is not currently provable since there is not restriction on what the fresh variables could be. I can change this so that the fresh variables are deterministic during adaptation *)
+Theorem adaptation_unique :
+  forall σ1 σ2 σ, σ1 ◁ σ2 ≜ σ ->
+             forall σ', σ1 ◁ σ2 ≜ σ' ->
+                   σ' = σ.
+Proof.
+  intros σ1 σ2 σ Hadapt1 σ' Hadapt2;
+    inversion Hadapt1;
+    inversion Hadapt2;
+    subst.
+  peek_pop_simpl; simpl in *.
+  inversion H; subst.
+  inversion H16; subst;
+    auto.
+Admitted.
+
+
+Ltac adapt_rewrite :=
+  repeat match goal with
+         | [H1 : ?σ1 ◁ ?σ2 ≜ ?σ, H2 : ?σ1 ◁ ?σ2 ≜ ?σ' |- _] =>
+           eapply (adaptation_unique σ1 σ2 σ H1) in H2;
+           eauto;
+           subst
+         end.
+
+Lemma pair_reductions_transitive :
+  forall M1 M2 σ1 σ2, M1 ⦂ M2 ⦿ σ1 ⤳⋆ σ2 ->
+                 forall σ3, M1 ⦂ M2 ⦿ σ2 ⤳⋆ σ3 ->
+                       M1 ⦂ M2 ⦿ σ1 ⤳⋆ σ3.
+Proof.
+  intros M1 M2 σ1 σ2 Hred;
+    induction Hred;
+    intros;
+    eauto.
+Qed.
